VerusLean/Json.lean
@@ -7,6 +7,16 @@ def isObject (j : Json) : Bool :=
   | Json.obj _ => true
   | _ => false
 
+def getNatUnderKey? (j : Json) (key : String) : Except String Nat := do
+  Json.getNat? <| ← j.getObjVal? key
+
+def getArrWithSizeGe? (j : Json) (n : Nat) : Except String ({ arr : Array Json // arr.size ≥ n }) := do
+  let arr ← j.getArr?
+  if h : arr.size ≥ n then
+    return ⟨arr, h⟩
+  else
+    throw s!"expected array of size {n}, got array of size {arr.size}"
+
 def getFirstValHelper? (j : Json) : List String → Except String (String × Json)
   | [] => throw "no keys matched"
   | k :: ks =>
@@ -21,12 +31,20 @@ def getFirstValHelper? (j : Json) : List String → Except String (String × Jso
 
   CC: Can be made faster by breaking the kvs API.
 -/
-def getFirstVal? (j : Json) (l : List String) : Except String (String × Json) :=
+def getFirstVal (j : Json) (l : List String) : Except String (String × Json) :=
   if j.isObject then
-    getFirstValHelper? j l
+    match getFirstValHelper? j l with
+    | .ok (s, v) => return (s, v)
+    | .error _ => throw s!"No keys matched. Expected one of {l}"
   else
     throw "object expected"
 
+/--
+  Gets a value underneath a "dot-path".
+
+  Acts like `getObjVal?`, except by chaining the elements in `path`
+  from left to right. If any one element fails, the whole query fails.
+-/
 def getObjValByPath (j : Json) (path : List String) : Except String Json :=
   match path with
   | [] => throw "empty path"
@@ -37,5 +55,34 @@ def getObjValByPath (j : Json) (path : List String) : Except String Json :=
       match j.getObjVal? k with
       | .ok v => getObjValByPath v ks
       | .error _ => throw "property not found"
+
+-- CC: Dunno how to set the priority of a notation, so we route all notation through `getFirstVal`
+-- Notation to alias a Json dictionary lookup
+--notation j "[" path "]" => Lean.Json.getObjVal? j path
+
+-- Notation to alias `getFirstVal`
+syntax term noWs "[" withoutPosition(sepBy(term, ", "))"]"  : term
+macro_rules
+  | `($j[ $elems,* ]) => do
+    let es := Syntax.TSepArray.getElems elems
+    match es.size with
+    | 1 => `(Lean.Json.getObjVal $j (es[0]))
+    | _ => `(Lean.Json.getFirstVal $j [ $elems,* ])
+
+
+/-def isInJson (j : Json) (key : String) : Prop :=
+  ∃ (val : Json), j.getObjVal? key = .ok val
+
+instance instGetElem : GetElem Json String Json isInJson where
+  getElem := fun j key h =>
+    match h_lookup : j.getObjVal? key with
+    | .ok v => v
+    | .error _ => by simp[isInJson, h_lookup] at h
+
+instance instGetElem? : GetElem? Json String Json isInJson where
+  getElem? := fun j key =>
+    match j.getObjVal? key with
+    | .ok v => some v
+    | .error _ => none -/
 
 end Lean.Json
