VerusLean/VLIR/Parser.lean
@@ -7,8 +7,8 @@ namespace VerusLean
 
 open Lean
 
-abbrev VMap := Std.HashMap String Typ
-abbrev FMap := Std.HashMap String SpecFn
+abbrev VMap := Std.HashMap Ident Typ
+abbrev FMap := Std.HashMap Ident SpecFn
 
 /--
   The parsing monad for Verus JSONs,
@@ -21,30 +21,109 @@ abbrev FMap := Std.HashMap String SpecFn
 
   TODO: handle shadowing
 -/
-abbrev VParser := EStateM String (Typ × VMap)
+structure ParserState where
+  expectedType : Typ := .Bool
+  freeVars : VMap := {}
+  -- Acts like a stack?
+  boundVars : List Ident := []
+  fns : FMap := {}
+deriving Inhabited
 
-def Typ.fromJson? (j : Json) : VParser Typ :=
-  -- dbg_trace s!"[Typ.fromJson?]: {j}"
+abbrev VParser := EStateM String ParserState
+
+/-- Alias for `Except String`. The argument following `ExStr` is the return type. -/
+abbrev ExStr := Except String
+
+namespace VParser
+
+open EStateM
+
+def getTyp : VParser Typ :=
+  do let st ← get; return st.expectedType
+
+def setTyp (t : Typ) : VParser Unit :=
+  modify fun st => { st with expectedType := t }
+
+def getFreeVars : VParser VMap :=
+  do let st ← get; return st.freeVars
+
+def getBoundVars : VParser (List Ident) :=
+  do let st ← get; return st.boundVars
+
+def addFreeVarWithTyp (var : Ident) (typ : Typ) : VParser Unit := do
+  modify fun st => { st with
+    freeVars := st.freeVars.insert var typ }
+
+def addFreeVar (var : Ident) : VParser Unit := do
+  addFreeVarWithTyp var (← getTyp)
+
+/--
+  Only adds a free variable if it is not already bound locally.
+-/
+def addFreeVarIfNotBound (var : Ident) : VParser Unit := do
+  if !(← getBoundVars).contains var then
+    addFreeVar var
+  else
+    return ()
+
+def pushBoundVar (var : Ident) : VParser Unit :=
+  modify fun st => { st with boundVars := var :: st.boundVars }
+
+def pushBoundVars (vars : List Ident) : VParser Unit :=
+  modify fun st => { st with boundVars := vars ++ st.boundVars }
+
+def popBoundVar : VParser Unit :=
+  modify fun st => { st with boundVars := st.boundVars.tail }
+
+def popBoundVars (n : Nat) : VParser Unit :=
+  modify fun st => { st with boundVars := st.boundVars.drop n }
+
+def withBoundVars (vars : List Ident) (fn : VParser α) : VParser α := do
+  pushBoundVars vars
+  let a ← fn
+  popBoundVars vars.length
+  return a
+
+def addSpecFn (fn : SpecFn) : VParser Unit :=
+  modify fun st => { st with fns := st.fns.insert fn.name fn }
+
+def setFns (fns : FMap) : VParser Unit :=
+  modify fun st => { st with fns := fns }
+
+def coeWithState : Except String α → VParser α
+  | .ok a => (fun s => Result.ok a s)
+  | .error e => (fun s => Result.error e s)
+
+instance instCoeExcept : Coe (Except String α) (VParser α) where
+  coe := coeWithState
+
+instance instCoeFunExcept {α : Type u} {β : Type} : Coe (α → ExStr β) (α → VParser β) where
+  coe f := fun a => f a
+
+end VParser
+
+--------------------------------------------------------------------------------
+
+open VParser
+
+def Typ.fromJson? (j : Json) : ExStr Typ := do
   match j.getStr? with
-  | .ok "Bool" => .ok Typ.Bool
+  | .ok "Bool" => return .Bool
   | .ok _ => throw "unsupported primitive type"
   | .error _ =>
-    match j.getFirstVal? ["Int", "Primitive", "ConstInt", "Array"] with
-    | .error e => throw s!"[Typ.fromJson? 1]: {e}, json is {j}"
-    | .ok ("Primitive", obj) =>
-      match obj.getArr? with
-      | .ok t => match t.get? 0 with
-        | some "Array" => throw "unsupported primitive type Array"
-        -- .ok (Typ.Array Typ.Int)
-        | some _ => throw "unsupported primitive type"
-        | none => throw s!"error, json: {obj}"
-        -- match Typ.fromJson? t with
-          -- | .ok Typ.Bool => .ok Typ.Bool
-          -- | .error e => throw s!"[Typ.fromJson? 3]: {e}"
-      | .error e => throw s!"{e}, json: {obj}"
-    -- | .ok ("Array", obj) => throw "Array ... not yet implemented"
-    -- | .ok ("ConstInt", obj) => throw "ConstInt not yet implemented"
-    | .ok ("Int", obj) =>
+    match ← j["Primitive", "Int", "ConstInt", "Array"] with
+    | ("Primitive", obj) =>
+      let t ← obj.getArr?
+      match t.get? 0 with
+      | some "Array" => throw "unsupported primitive type Array"
+      -- .ok (Typ.Array Typ.Int)
+      | some _ => throw "unsupported primitive type"
+      | none => throw s!"error, json: {obj}"
+      -- match Typ.fromJson? t with
+        -- | .ok Typ.Bool => .ok Typ.Bool
+        -- | .error e => throw s!"[Typ.fromJson? 3]: {e}"
+
+    | ("Int", obj) =>
       -- First, we check if the the underlying string is "Int" for mathematical integers
       match obj.getStr? with
       | .ok "Int" => .ok Typ.Int
@@ -52,7 +131,7 @@ def Typ.fromJson? (j : Json) : VParser Typ :=
       | .ok _ => throw s!"unsupported Int object string: {obj}"
       | .error _ =>
         -- Now check if it is a fixed-width integer
-        match obj.getFirstVal? ["U", "I"] with
+        match obj.getFirstVal ["U", "I"] with
         | .error _ => throw s!"unsupported Int object: {obj}"
         | .ok ("U", obj) =>
           match obj.getNat? with
@@ -64,7 +143,7 @@ def Typ.fromJson? (j : Json) : VParser Typ :=
           | .error e => throw s!"[Typ.fromJson?]: {e}"
         | .ok _ => throw s!"unsupported Int object: {obj}"
 
-    | .ok _ => throw "unsupported primitive type"
+    | _ => throw "unsupported primitive type"
 
 /--
   Parses a "span" object and forwards the underlying data to a given function `fj`.
@@ -72,340 +151,235 @@ def Typ.fromJson? (j : Json) : VParser Typ :=
   Also adds the type annotation for the span to the state.
   This annotation should be added to the state's `HashMap` when encountering a `Var`.
 -/
-def fromJsonSpanned? {α : Type} (j : Json) (fj : Json → VParser α) : VParser α :=
-  match j.getObjVal? "span" with
-  | .error e => throw s!"[fromJsonSpanned?]: no span found: {e}"
-  | .ok _ => do
-    match j.getObjVal? "typ" with
-    | .error _ => throw "[fromJsonSpanned?]: no typ found"
-    | .ok obj => do
-      let typ ← Typ.fromJson? obj
-      match j.getObjVal? "x" with
-      | .error e => throw s!"[fromJsonSpanned?]: no x found: {e}"
-      | .ok x => (fun (_, map) => fj x (typ, map))
+def fromJsonSpanned? {α : Type} (j : Json) (fj : Json → VParser α) : VParser α := do
+  let typ ← Typ.fromJson? <| ← j.getObjVal? "typ"
+  let x ← j.getObjVal? "x"
+  setTyp typ
+  fj x
 
-def xJsonFromSpanned? (j : Json) : VParser Json :=
-  match j.getObjVal? "span" with
-  | .error e => throw s!"[xFromJsonSpanned?]: no span found: {e}"
-  | .ok _ => j.getObjVal? "x"
+def xJsonFromSpanned? (j : Json) : ExStr Json :=
+  j.getObjVal? "x"
 
-def typFromX? (j : Json) : VParser Typ :=
-  match j.getObjVal? "typ" with
-  | .error e => throw s!"[typFromX?]: {e} with json {j}"
-  | .ok obj => Typ.fromJson? obj
+def typFromX? (j : Json) : ExStr Typ := do
+  Typ.fromJson? <| ← j.getObjValByPath ["x", "typ"]
 
-def nameTypFromX? (j : Json) : VParser (String × Typ) :=
-  match j.getObjVal? "name" with
-  | .error e => throw s!"[nameTypFromX?]: {e}"
-  | .ok obj => do
-    match obj.getArr? with
-    | .error e => throw s!"[nameTypFromX?]: {e}"
-    | .ok arr => do
-      if h : arr.size < 1 then
-        throw s!"[nameTypFromX?]: Expected an array of size at least 1, got {arr.size}"
-      else
-        let name := arr.get 0 (by omega)
-        match name.getStr? with
-        | .ok name =>
-          let typ ← typFromX? j
-          return (name, typ)
-        | .error e => throw s!"[nameTypFromX?]: {e}"
+def widthFromJson? (j : Json) : ExStr Nat := do
+  j.getNatUnderKey? "Width"
 
-def widthFromJson? (j : Json) : VParser Nat :=
-  match j.getObjVal? "Width" with
-  | .error e => throw s!"[widthFromJson]: {e}"
-  | .ok w =>
-    match w.getNat? with
-    | .ok width => .ok width
-    | .error e => throw s!"[widthFromJson]: {e}"
+-- TODO: This probably needs to return a namespace (list?), rather than a single ident
+def pathedNameFromJson? (j : Json) : ExStr Ident := do
+  let pathed ← j.getObjValByPath ["path", "segments"]
+  Json.getStr? <| ← Json.getArrVal? pathed 0
 
-def Mode.fromJson? (j : Json) : VParser Mode :=
-  match j.getStr? with
-  | .ok "Spec" => .ok Mode.Spec
-  | .ok "Proof" => .ok Mode.Proof
-  | .ok "Exec" => .ok Mode.Exec
-  | .ok str => throw s!"[Mode.fromJson?]: Expected one of \{ Spec, Proof, Exec }, got {str}"
-  | .error e => throw s!"[Mode.fromJson?]: {e}"
+--------------------------------------------------------------------------------
 
-def Const.fromJson? (j : Json) : VParser Const :=
-  match j.getFirstVal? ["Bool", "Int", "StrSlice", "Char"] with
-  | .error _ => throw "[Const.fromJson?] Expected a JSON object under one of the const keys"
-  | .ok ("Bool", v) =>
-    match v.getBool? with
-    | .ok b => .ok (Const.Bool b)
-    | .error e => throw s!"[Const.fromJson?]: {e}"
-  | .ok ("Int", v) =>
+def Mode.fromJson? (j : Json) : ExStr Mode := do
+  match ← j.getStr? with
+  | "Spec"  => return .Spec
+  | "Proof" => return .Proof
+  | "Exec"  => return .Exec
+  | str => throw s!"[Mode.fromJson?]: Expected one of \{ Spec, Proof, Exec }, got {str}"
+
+def Const.fromJson? (j : Json) : ExStr Const := do
+  match ← j["Bool", "Int", "StrSlice", "Char"] with
+  | ("Bool", v) => return Const.Bool <| ← v.getBool?
+  | ("Int", v) =>
     -- Ints are serialized as an array, with the first element the sign enum
     -- and the second value is the data, an array of u64s.
-    match v.getArr? with
-    | .error e => throw s!"[Const.fromJson?]: {e}"
-    | .ok arr =>
-      if h : arr.size < 2 then
-        throw s!"[Const.fromJson?]: Expected an array of size at least 2, got {arr.size}"
-      else
-        match arr.get 0 (by omega), arr.get 1 (by omega) with
-        | s, n =>
-          match s.getNat? with
-          | .error e => throw s!"[Const.fromJson?]: {e}"
-          | .ok 0 => -- no sign -- CZ: according to bigint.rs, 0 is minus, 1 is no sign, 2 is plus?
-            .ok (Const.Int 0)
-          | .ok 1 => -- positive number
-            match n.getArr? with
-            | .error e => throw s!"[Const.fromJson?]: {e}"
-            | .ok n =>
-              -- TODO: Need some computation for the big int
-              -- For now, take the first entry and move on
-              let n := n.getD 0 (Json.num <| JsonNumber.fromNat 0)
-              match n.getNat? with
-              | .ok i => .ok (Const.Int i)
-              | .error e => throw s!"[Const.fromJson?]: {e}"
-          | .ok 2 => -- negative number
-            match n.getArr? with
-            | .error e => throw s!"[Const.fromJson?]: {e}"
-            | .ok n =>
-              -- TODO: Need some computation for the big int
-              -- For now, take the first entry and move on
-              let n := n.getD 0 (Json.num <| JsonNumber.fromNat 0)
-              match n.getNat? with
-              | .ok i => .ok (Const.Int <| -(Int.ofNat i))
-              | .error e => throw s!"[Const.fromJson?]: {e}"
-          | .ok _ => throw "[Const.fromJson?]: Expected an Int sign of 0, 1, or 2"
-  | .ok ("StrSlice", _) => throw "not yet implemented"
-  | .ok ("Char", _) => throw "not yet implemented"
+    let ⟨arr, _⟩ ← v.getArrWithSizeGe? 2
+    let s := arr[0]
+    let n := arr[1]
+    match ← s.getNat? with
+    | 0 =>
+      -- no sign
+      -- CZ: according to bigint.rs, 0 is minus, 1 is no sign, 2 is plus?
+      .ok (Const.Int 0)
+    | 1 =>
+      -- positive number
+      -- TODO: Need some computation for the big int
+      -- For now, take the first entry and move on
+      let nArr ← n.getArr?
+      let n := nArr.getD 0 (Json.num <| JsonNumber.fromNat 0)
+      return Const.Int <| Int.ofNat <| ← n.getNat?
+    | 2 =>
+      -- negative number
+      -- TODO: Need some computation for the big int
+      -- For now, take the first entry and move on
+      let nArr ← n.getArr?
+      let n := nArr.getD 0 (Json.num <| JsonNumber.fromNat 0)
+      return Const.Int <| -(Int.ofNat <| ← n.getNat?)
+    | _ => throw "[Const.fromJson?]: Expected an Int sign of 0, 1, or 2"
+  | ("StrSlice", _) => throw "not yet implemented"
+  | ("Char", _) => throw "not yet implemented"
   | _ => throw "[Const.fromJson?]: Unexpected match"
 
-def Bitwise.fromJson? (j : Json) : VParser BitwiseOp :=
+def Bitwise.fromJson? (j : Json) : ExStr BitwiseOp :=
   match j.getStr? with
-  | .ok "BitXor" => .ok BitwiseOp.BitXor
-  | .ok "BitAnd" => .ok BitwiseOp.BitAnd
-  | .ok "BitOr" => .ok BitwiseOp.BitOr
+  | .ok "BitXor" => return .BitXor
+  | .ok "BitAnd" => return .BitAnd
+  | .ok "BitOr"  => return .BitOr
   | .ok str => throw s!"[Bitwise.fromJson?]: Expected one of \{ BitXor, BitAnd, BitOr }, got {str}"
-  | .error _ =>
+  | .error _ => do
     -- Try one of the shifts instead
-    -- They are objects that store the width (and sign extension)
-    match j.getFirstVal? ["Shr", "Shl"] with
-    | .ok ("Shr", obj) => do
+    -- They are Json objects that store the width (and sign extension)
+    match ← j["Shr", "Shl"] with
+    | ("Shr", obj) => do
       let width ← widthFromJson? obj
-      return BitwiseOp.Shr width
+      return .Shr width
 
-    | .ok ("Shl", obj) =>
-      match obj.getArr? with
-      | .error e => throw s!"[Bitwise.fromJson?]: {e}"
-      | .ok arr => do
-        if h : arr.size < 2 then
-          throw s!"[Bitwise.fromJson?]: Expected an array of size at least 2, got {arr.size}"
-        else
-          let widthObj := arr.get 0 (by omega)
-          let signExtend := arr.get 1 (by omega)
-          let width ← widthFromJson? widthObj
-          match signExtend.getBool? with
-          | .ok signExtend => .ok (BitwiseOp.Shl width signExtend)
-          | .error e => throw s!"[Bitwise.fromJson?]: {e}"
+    | ("Shl", obj) =>
+      let ⟨arr, _⟩ ← obj.getArrWithSizeGe? 2
+      let width ← widthFromJson? arr[0]
+      return .Shl width (← arr[1].getBool?)
 
     | _ => throw s!"[Bitwise.fromJson?]: Expected one of \{ Shr, Shl }, got {j}"
 
-def ArithOp.fromJson? (j : Json) : VParser ArithOp :=
-  match j.getStr? with
-  | .ok "Add" => .ok ArithOp.Add
-  | .ok "Sub" => .ok ArithOp.Sub
-  | .ok "Mul" => .ok ArithOp.Mul
-  | .ok "EuclideanDiv" => .ok ArithOp.EuclideanDiv
-  | .ok "EuclideanMod" => .ok ArithOp.EuclideanMod
-  | .ok str => throw s!"[ArithOp.fromJson?]: Expected one of Add, Sub, Mul, Div, Mod, got {str}"
-  | .error e => throw s!"[ArithOp.fromJson?]: {e}"
+def ArithOp.fromJson? (j : Json) : ExStr ArithOp := do
+  match ← j.getStr? with
+  | "Add"          => return .Add
+  | "Sub"          => return .Sub
+  | "Mul"          => return .Mul
+  | "EuclideanDiv" => return .EuclideanDiv
+  | "EuclideanMod" => return .EuclideanMod
+  | s => throw s!"[ArithOp.fromJson?]: Expected one of Add, Sub, Mul, Div, Mod, got {s}"
 
-def InequalityOp.fromJson? (j : Json) : VParser InequalityOp :=
-  match j.getStr? with
-  | .ok "Le" => .ok InequalityOp.Le
-  | .ok "Ge" => .ok InequalityOp.Ge
-  | .ok "Lt" => .ok InequalityOp.Lt
-  | .ok "Gt" => .ok InequalityOp.Gt
-  | .ok s => throw s!"[InequalityOp.fromJson?]: Expected one of \{ Le, Ge, Lt, Gt }, got {s}"
-  | .error e => throw s!"[InequalityOp.fromJson?]: {e}"
+def InequalityOp.fromJson? (j : Json) : ExStr InequalityOp := do
+  match ← j.getStr? with
+  | "Le" => return .Le
+  | "Ge" => return .Ge
+  | "Lt" => return .Lt
+  | "Gt" => return .Gt
+  | s => throw s!"[InequalityOp.fromJson?]: Expected one of \{ Le, Ge, Lt, Gt }, got {s}"
 
-def UnaryOp.fromJson? (j : Json) : VParser UnaryOp :=
-  -- dbg_trace s!"[UnaryOp.fromJson?]: {j}"
+def UnaryOp.fromJson? (j : Json) : ExStr UnaryOp :=
   match j.getStr? with
-  | .ok "Not" => .ok UnaryOp.Not
+  | .ok "Not"    => return .Not
   | .ok "BitNot" => throw "not yet implemented"
-  | .ok "Clip" => throw "not yet implemented"
+  | .ok "Clip"   => throw "not yet implemented"
   | .ok s => throw s!"[UnaryOp.fromJson?]: Expected one of \{ Not, BitNot, Clip }, got {s}"
-  | .error _ =>
+  | .error _ => do
     -- Try seeing if "BitNot" has a width
-    match j.getObjVal? "BitNot" with
-    | .ok obj => do
-      let width ← widthFromJson? obj
-      return UnaryOp.BitNot width
-    | .error e =>
-      -- throw s!"[UnaryOp.fromJson?]: {e}"
-      -- Try seeing if it's a trigger
-      match j.getObjVal? "Trigger" with
-      | .error e => throw s!"[UnaryOp.fromJson?]: {e}"
-      | .ok _ => .ok UnaryOp.Trigger
-        -- match j.getArrVal? 1 with
-        -- | .error e => throw s!"expected an array of size 2: {e}, with json {j}"
-        -- | .ok obj => do
-        --   let obj ← fromJsonSpanned? obj ExpX.fromJson?
-        --   return UnaryOp.Trigger obj
+    let obj ← j.getObjVal? "BitNot"
+    let width ← widthFromJson? obj
+    return .BitNot width
 
-def BinaryOp.fromJson? (j : Json) : VParser BinaryOp :=
+def BinaryOp.fromJson? (j : Json) : ExStr BinaryOp :=
   -- Most are single strings, but Eq has a mode attached, etc.
   match j.getStr? with
-  | .ok "And" => .ok BinaryOp.And
-  | .ok "Or" => .ok BinaryOp.Or
-  | .ok "Xor" => .ok BinaryOp.Xor
-  | .ok "Implies" => .ok BinaryOp.Implies
-  | .ok "Ne" => .ok BinaryOp.Ne
+  | .ok "And"     => return .And
+  | .ok "Or"      => return .Or
+  | .ok "Xor"     => return .Xor
+  | .ok "Implies" => return .Implies
+  | .ok "Ne"      => return .Ne
   | .ok s => throw s!"[BinaryOp.fromJson?]: Expected one of \{ And, Or, Xor, Implies, Ne }, got {s}"
-  | .error _ =>
+  | .error _ => do
     -- Try one of the object ops instead
-    match j.getFirstVal? ["Eq", "Inequality", "Bitwise", "Arith"] with
-    | .ok ("Eq", obj) => do return BinaryOp.Eq (← Mode.fromJson? obj)
-    | .ok ("Inequality", obj) => do return BinaryOp.Inequality (← InequalityOp.fromJson? obj)
-    | .ok ("Bitwise", obj) =>
+    match ← j["Eq", "Inequality", "Bitwise", "Arith"] with
+    | ("Eq", obj)         => return .Eq (← Mode.fromJson? obj)
+    | ("Inequality", obj) => return .Inequality (← InequalityOp.fromJson? obj)
+    | ("Bitwise", obj) =>
       -- Object under "Bitwise" should be a two-element array with an op and a mode
-      match obj.getArr? with
-      | .error e => throw s!"[BinaryOp.fromJson?]: {e}"
-      | .ok arr => do
-        if h : arr.size < 2 then
-          throw s!"[BinaryOp.fromJson?]: Expected an array of size at least 2, got {arr.size}"
-        else
-          let op := arr.get 0 (by omega)
-          let mode := arr.get 1 (by omega)
-          let op ← Bitwise.fromJson? op
-          let mode ← Mode.fromJson? mode
-          return BinaryOp.Bitwise op mode
-    | .ok ("Arith", obj) =>
+      let ⟨arr, _⟩ ← obj.getArrWithSizeGe? 2
+      let op ← Bitwise.fromJson? arr[0]
+      let mode ← Mode.fromJson? arr[1]
+      return .Bitwise op mode
+    | ("Arith", obj) =>
       -- Object under "Arith" should be a two-element array with an op and a mode
-      match obj.getArr? with
-      | .error e => throw s!"[BinaryOp.fromJson?]: {e}"
-      | .ok arr => do
-        if h : arr.size < 2 then
-          throw s!"[BinaryOp.fromJson?]: Expected an array of size at least 2, got {arr.size}"
-        else
-          let op := arr.get 0 (by omega)
-          let mode := arr.get 1 (by omega)
-          let op ← ArithOp.fromJson? op
-          let mode ← Mode.fromJson? mode
-          return BinaryOp.Arith op mode
+      let ⟨arr, _⟩ ← obj.getArrWithSizeGe? 2
+      let op ← ArithOp.fromJson? arr[0]
+      let mode ← Mode.fromJson? arr[1]
+      return .Arith op mode
     | _ => throw s!"[BinaryOp.fromJson?]: Expected one of \{ And, Or, Xor, Implies, Eq }, got something else: {j}"
 
-def Quant.fromJson? (j : Json) : VParser Quant :=
-  match j.getObjVal? "quant" with
-  | .ok "Forall" => .ok Quant.Forall
-  | .ok "Exists" => .ok Quant.Exists
-  | .ok s => throw s!"[Quant.fromJson?]: Expected one of \{ Forall, Exists }, got {s}"
-  | .error e => throw s!"[Quant.fromJson?]: {e}, with json {j}"
+def Quant.fromJson? (j : Json) : ExStr Quant := do
+  match ← j.getObjVal? "quant" with
+  | "Forall" => return .Forall
+  | "Exists" => return .Exists
+  | s => throw s!"[Quant.fromJson?]: Expected one of \{ Forall, Exists }, got {s}"
 
-def varBinderFromJson? (j : Json) : VParser (String × Typ) :=
-  match j.getObjVal? "name" with
-  | .error e => throw s!"[varBinderFromJson?]: no name found: {e}"
-  | .ok obj => do
-    match obj.getArr? with
-    | .error e => throw s!"[varBinderFromJson?]: {e}"
-    | .ok arr => do
-      if h : arr.size < 1 then
-        throw s!"[varBinderFromJson?]: Expected an array of size at least 1, got {arr.size}"
-      else
-        let name := arr.get 0 (by omega)
-        match name.getStr? with
-        | .ok name =>
-          match j.getObjVal? "a" with
-          | .error e => throw s!"[varBinderFromJson?]: no type found: {e}"
-          | .ok typ => do
-            -- dbg_trace s!"[varBinderFromJson?]: name={name}, typ={typ}"
-            let typ ← Typ.fromJson? typ
-            return (name, typ)
-          -- throw s!"[varBinderFromJson?]: {name} not yet implemented"
-          -- let typ ← Typ.fromJson? typ
-          -- return (name, typ)
-        | .error e => throw s!"[varBinderFromJson?]: {e}"
+def CallFun.fromJson? (j : Json) : ExStr CallFun := do
+  let obj ← j.getObjVal? "Fun"
+  let ⟨arr, _⟩ ← obj.getArrWithSizeGe? 1
+  return .Fun (← pathedNameFromJson? arr[0])
 
-def VarBinders.fromJson? (j : Json) : VParser VarBinders :=
-  match j.getArr? with
-  | .error e => throw s!"[VarBinders.fromJson?]: {e}"
-  | .ok arr => arr.toList.mapM varBinderFromJson?
+def VarBinder.typFromJson? (j : Json) : ExStr (VarBinder Typ) := do
+  let obj ← j.getObjVal? "name"
+  let ⟨arr, _⟩ ← obj.getArrWithSizeGe? 1
+  let name ← arr[0].getStr?
+  let typ ← typFromX? j
+  return VarBinder.mk name typ
 
-def Bind.fromJson? (j : Json) : VParser Bind := do
+def VarBinder.typBinderFromJson? (j : Json) : ExStr (VarBinder Typ) := do
+  let obj ← j.getObjVal? "name"
+  let ⟨arr, _⟩ ← obj.getArrWithSizeGe? 1
+  let nameObj := arr[0]
+  let (name : String) ← nameObj.getStr?
+  let typ ← Typ.fromJson? (← j.getObjVal? "typ")
+  return VarBinder.mk name typ
+
+def VarBinder.typBindersFromJson? (j : Json) : ExStr (List (VarBinder Typ)) := do
+  let (arr : _root_.Array Json) ← j.getArr?
+  arr.toList.mapM VarBinder.typBinderFromJson?
+
+mutual /- {Bind, Exp}.fromJson? -/
+
+partial def Bind.fromJson? (j : Json) : VParser Bind := do
   let obj : Json ← xJsonFromSpanned? j
-  match obj.getObjVal? "Quant" with
-  | .error e => throw s!"[Bind.fromJson?]: {e}"
-  | .ok arr =>
-    match arr.getArr? with
-    | .error e => throw s!"[Bind.fromJson?]: {e}"
-    | .ok arr => do
-      if h : arr.size < 4 then
-        throw s!"[Bind.fromJson?]: Expected an array of size at least 4, got {arr.size}"
-      else
-        let q := arr.get 0 (by omega)
-        let binders := arr.get 1 (by omega)
-        -- let trigs := arr.get 2 (by omega)
-        -- let AssertByLocals := arr.get 3 (by omega)
-        let q ← Quant.fromJson? q
-        let binders ← VarBinders.fromJson? binders
-        return Bind.Quant q binders
+  match ← obj.getFirstVal ["Quant"] with
+  | ("Quant", (q : Json)) =>
+    let ⟨arr, _⟩ ← coeWithState <| q.getArrWithSizeGe? 4
+    let q ← Quant.fromJson? arr[0]
+    let binders ← VarBinder.typBindersFromJson? arr[1]
+    return .Quant q binders
+  | _ => throw "unexpected"
 
-partial def ExpX.fromJson? (j : Json) : VParser ExpX :=
+partial def Exp.fromJson? (j : Json) : VParser Exp := do
   -- Expect that exactly one of the enumerated options will be true
-  match j.getFirstVal? ["Const", "Var", "Unary", "Binary", "If", "Array", "Bind", "Call"] with
-  | .ok ("Const", obj) => do
-    let c ← Const.fromJson? obj
-    return ExpX.Const c
-  | .ok ("Var", obj) =>
+  match ← j["Const", "Var", "Unary", "Binary", "If", "Bind", "Call"] with
+  | ("Const", obj) => do
+    return Exp.Const <| ← Const.fromJson? obj
+  | ("Var", obj) =>
     -- Verus gives us an array, where the first element is the identifier
-    match obj.getArrVal? 0 with
-    | .error e => throw s!"[ExpX.fromJson?] 1: {e}"
-    | .ok i =>
-      match i.getStr? with
-      | .error e => throw s!"[ExpX.fromJson?] 2: {e}"
-      | .ok ident =>
-        -- Add the variable to the state's map
-        (fun (typ, map) =>
-          let map := map.insert ident typ
-          .ok (ExpX.Var ident) (typ, map))
-  | .ok ("Unary", obj) =>
+    let (i : Json) ← obj.getArrVal? 0
+    let (ident : Ident) ← i.getStr?
+    addFreeVarIfNotBound ident
+    return .Var ident
+  | ("Unary", obj) =>
     -- A unary object should be an array with an op and a data element
-    match obj.getArr? with
-    | .error e => throw s!"[ExpX.fromJson?] 3: {e}"
-    | .ok arr => do
-      if h : arr.size < 2 then
-        throw s!"[ExpX.fromJson?]: Expected an array of size at least 2, got {arr.size}"
-      else
-        let op := arr.get 0 (by omega)
-        let data := arr.get 1 (by omega)
-        let op ← UnaryOp.fromJson? op
-        let data ← fromJsonSpanned? data ExpX.fromJson?
-        return ExpX.Unary op data
-  | .ok ("Binary", obj) =>
+    let ⟨arr, _⟩ ← coeWithState <| obj.getArrWithSizeGe? 2
+    let op   ← UnaryOp.fromJson? arr[0]
+    let data ← fromJsonSpanned? arr[1] Exp.fromJson?
+    return .Unary op data
+  | ("Binary", obj) =>
     -- A binary object should be an array with an op and two data elements
-    match obj.getArr? with
-    | .error e => throw s!"[ExpX.fromJson?] 4: {e}"
-    | .ok arr => do
-      if h : arr.size < 3 then
-        throw s!"[ExpX.fromJson?]: Expected an array of size at least 3, got {arr.size}"
-      else
-        let op := arr.get 0 (by omega)
-        let data₁ := arr.get 1 (by omega)
-        let data₂ := arr.get 2 (by omega)
-        let op ← BinaryOp.fromJson? op
-        let data₁ ← fromJsonSpanned? data₁ ExpX.fromJson?
-        let data₂ ← fromJsonSpanned? data₂ ExpX.fromJson?
-        return ExpX.Binary op data₁ data₂
-  | .ok ("If", obj) =>
+    let ⟨arr, _⟩ ← coeWithState <| obj.getArrWithSizeGe? 3
+    let op    ← BinaryOp.fromJson? arr[0]
+    let data₁ ← fromJsonSpanned? arr[1] Exp.fromJson?
+    let data₂ ← fromJsonSpanned? arr[2] Exp.fromJson?
+    return .Binary op data₁ data₂
+  | ("If", obj) =>
     -- Should be an array with three expressions
-    match obj.getArr? with
-    | .error e => throw s!"[ExpX.fromJson?] 5: {e}"
-    | .ok arr => do
-      if h : arr.size < 3 then
-        throw s!"[ExpX.fromJson?]: Expected an array of size at least 3, got {arr.size}"
-      else
-        let cond := arr.get 0 (by omega)
-        let branch₁ := arr.get 1 (by omega)
-        let branch₂ := arr.get 2 (by omega)
-        let cond ← fromJsonSpanned? cond ExpX.fromJson?
-        let branch₁ ← fromJsonSpanned? branch₁ ExpX.fromJson?
-        let branch₂ ← fromJsonSpanned? branch₂ ExpX.fromJson?
-        return ExpX.If cond branch₁ branch₂
+    let ⟨arr, _⟩ ← coeWithState <| obj.getArrWithSizeGe? 3
+    let cond    ← fromJsonSpanned? arr[0] Exp.fromJson?
+    let branch₁ ← fromJsonSpanned? arr[1] Exp.fromJson?
+    let branch₂ ← fromJsonSpanned? arr[2] Exp.fromJson?
+    return .If cond branch₁ branch₂
+  | ("Bind", obj) =>
+    -- Should be an array with a bind and an expression
+    let ⟨arr, _⟩ ← coeWithState <| obj.getArrWithSizeGe? 2
+    let bind ← Bind.fromJson? arr[0]
+    let exp ← withBoundVars bind.idents (fromJsonSpanned? arr[1] Exp.fromJson?)
+    return .Bind bind exp
+  | ("Call", obj) =>
+    -- Should be an object with a function name and arguments
+    -- The function's name is the 0th element, the arguments the 2nd element (an array)
+    let ⟨arr, _⟩ ← coeWithState <| obj.getArrWithSizeGe? 3
+    let callFn ← CallFun.fromJson? arr[0]
+    let (expsJson : Array Json) ← arr[2].getArr?
+    let exps : Array Exp ← expsJson.mapM (fromJsonSpanned? · Exp.fromJson?)
+    return .Call callFn [] exps.toList
+  | s => throw s!"[ExpX.fromJson?]: Expected one of \{ Const, Var, Unary, Binary, If }, got {s}"
+
   -- | .ok ("Array", obj) =>
   --   -- Should be an array of expressions
   --   match obj.getArr? with
@@ -413,75 +387,47 @@ partial def ExpX.fromJson? (j : Json) : VParser ExpX :=
   --   | .ok arr => do
   --     let elems ← arr.mapM (fun i => fromJsonSpanned? i ExpX.fromJson?)
   --     return ExpX.ArrayLiteral elems
-  | .ok ("Bind", obj) =>
-    -- Should be an array with a bind and an expression
-    match obj.getArr? with
-    | .error e => throw s!"[ExpX.fromJson?] 6: {e}"
-    | .ok arr => do
-      if h : arr.size < 2 then
-        throw s!"[ExpX.fromJson?]: Expected an array of size at least 2, got {arr.size}"
-      else
-        let bind := arr.get 0 (by omega)
-        let exp := arr.get 1 (by omega)
-        -- throw s!"bind: {bind}, exp: {exp}"
-        let bind ← Bind.fromJson? bind
-        let exp ← fromJsonSpanned? exp ExpX.fromJson?
-        return ExpX.Bind bind exp
-  | .ok ("Call", obj) =>
-    -- Should be an object with a function name and arguments
-    match obj.getArr? with
-    | .error e => throw s!"[ExpX.fromJson?] b {e}"
-    | .ok arr => do
-      if h : arr.size < 3 then
-        throw s!"[ExpX.fromJson?]: Expected an array of size at least 2, got {arr.size}"
-      else
-        let fn := arr.get 0 (by omega)
-        -- let typs := arr.get 1 (by omega)
-        let exps := arr.get 2 (by omega)
 
-        let fnJson : Json ← fn.getObjVal? "Fun"
-        let fnJson : Json ← fnJson.getArrVal? 0
-        let fnSeg : Json ← fnJson.getObjValByPath ["path", "segments"]
-        let fnName : Json ← fnSeg.getArrVal? 0
-        let fnStr : String ← fnName.getStr?
+end /- mutual -/
 
-        let expsJson : Array Json ← exps.getArr?
-        let exps : Array ExpX ← expsJson.mapM (fun i => fromJsonSpanned? i ExpX.fromJson?)
-        return ExpX.Call (CallFun.Fun fnStr) [] exps.toList
-    -- throw s!"call not yet implemented, obj is {j}"
-  | .ok _ => throw "[ExpX.fromJson?]: Expected one of { Const, Var, Unary, Binary, If }, got something else"
-  | .error e => throw s!"[ExpX.fromJson?] 7: {e}, json is {j}"
+--------------------------------------------------------------------------------
 
-partial def ExpX.fromFile? (path : String) : IO (Except String (ExpX × VMap)) := do
+/-partial def Exp.fromFile? (path : String) : IO (Except String (Exp × VMap)) := do
   let jsonStr ← IO.FS.readFile path
   let json ← IO.ofExcept <| Json.parse jsonStr
-  match ExpX.fromJson? json (.Bool, Std.HashMap.empty) with
+  match Exp.fromJson? json with
   | .ok exp (_, types) => return .ok (exp, types)
-  | .error e _ => return .error e
+  | .error e _ => return .error e -/
 
-def getSpecFnName? (j : Json) : VParser String := do
+def getSpecFnName? (j : Json) : ExStr String := do
   let obj : Json ← j.getObjValByPath ["x", "name", "path", "segments"]
-  match obj.getArrVal? 0 with
-  | .error e => throw s!"[getSpecFnName?]: {e}"
-  | .ok segments => return ← segments.getStr?
+  Json.getStr? <| ← obj.getArrVal? 0
 
-def SpecFn.fromJson? (j : Json) : VParser SpecFn := do
+def SpecFn.fromJson? (j : Json) : ExStr SpecFn := do
   let name ← getSpecFnName? j
-  let inputsJson : Json ← j.getObjValByPath ["x", "pars"]
-  let inputsJson : Array Json := (Json.getArr? inputsJson).toOption.getD #[]
-  let inputsDefs ← inputsJson.mapM (
-    fun i => do nameTypFromX? (← xJsonFromSpanned? i)
-  )
-  let mut inputs : Std.HashMap Ident Typ := Std.HashMap.empty
-  for (name, typ) in inputsDefs do
-    inputs := inputs.insert name typ
-  let returnTypeJson : Json ← j.getObjValByPath ["x", "ret"]
-  let returnType : Typ ← typFromX? (← xJsonFromSpanned? returnTypeJson)
-  let body : Json ← j.getObjValByPath ["x", "axioms", "spec_axioms", "body_exp"]
-  -- dbg_trace s!"[SpecFn.fromJson?]: body: {body}"
-  return SpecFn.mk name inputs returnType (← fromJsonSpanned? body ExpX.fromJson?)
 
-abbrev Decls := List Decl
+  -- Parse the arguments
+  let inputsJson ← j.getObjValByPath ["x", "pars"]
+  let varsArr ← inputsJson.getArr?
+  let vars ← varsArr.foldlM (init := Std.HashMap.empty) (fun m v => do
+    let (var : VarBinder Typ) ← VarBinder.typBinderFromJson? (← xJsonFromSpanned? v)
+    return m.insert (VarBinder.name var) (VarBinder.val var)
+  )
+
+  -- Parse the return type
+  let returnTypeJson : Json ← j.getObjValByPath ["x", "ret"]
+  let returnType : Typ ← typFromX? returnTypeJson
+
+  -- Parse the body as an expression
+  let bodyObj : Json ← j.getObjValByPath ["x", "axioms", "spec_axioms", "body_exp"]
+  match fromJsonSpanned? bodyObj Exp.fromJson? {
+      expectedType := returnType
+      freeVars := vars
+      boundVars := ∅
+      fns := Std.HashMap.empty -- CC: TODO this probably gets accumulated as we parse?
+    } with
+  | .ok body _ => return SpecFn.mk name vars returnType body
+  | .error e _ => throw e
 
 /--
   Parses a JSON into a `Decl`, or throws an error.
@@ -494,49 +440,42 @@ abbrev Decls := List Decl
   This function will try to parse an assert first, and if that fails,
   tries to parse a function.
 -/
-partial def Decls.fromJson? (j : Json) : VParser Decls :=
-  -- dbg_trace s!"[Decl.fromJson?]: {j}"
-  match j.getFirstVal? ["Assert", "FuncCheckSST"] with
-  | .ok ("Assert", obj) => do
-    let mut res : Decls := []
-    -- dbg_trace s!"[Decl.fromJson?]: Assert object: {obj}"
-    let exp ← ExpX.fromJson? obj
-    let (_, vmap) ← get
-    let specFnsJson : Json ← j.getObjVal? "SpecFns"
-    let specFns := (Json.getArr? specFnsJson).toOption.getD #[]
-    -- let fmap : FMap := Std.HashMap.empty
-    -- dbg_trace s!"[Decl.fromJson?]: get here"
+partial def Decl.fromJson? (j : Json) : VParser Decl := do
+  match ← j["Assert", "FuncCheckSST"] with
+  | ("Assert", (obj : Json)) =>
+    -- Parse the spec functions
+    let specObjs ← coeWithState <| Json.getArr? <| ← j.getObjVal? "SpecFns"
+    let fnMap ← specObjs.foldlM (init := ∅) (fun m fnJson => do
+      let fn ← SpecFn.fromJson? fnJson
+      return Std.HashMap.insert m (SpecFn.name fn) fn
+    )
 
-    for specFnJson in specFns do
-      -- dbg_trace s!"specFnJson: {specFnJson}"
-      let specFnName ← getSpecFnName? specFnJson
-      let specFn ← SpecFn.fromJson? specFnJson
-      -- let fmap := fmap.insert specFnName specFn
-      let specfnDecl := Decl.specfn specFnName specFn.inputs specFn.returnType specFn.body
-      -- dbg_trace s!"specfnDecl: {specfnDecl}"
-      res := res.append [specfnDecl]
+    -- CC: TODO we probably shouldn't manually set the functions here (add them?)
+    setFns fnMap
 
-    let assertIdJson ← j.getObjVal? "AssertId"
-    let assertId : Nat ← Json.getNat? assertIdJson
-    let actualAssert := Decl.assertion s!"assert_{assertId}" vmap exp
-    res := res.append [actualAssert]
-    return res
+    -- Parse the body of the assert, now that we have the spec functions
+    let exp ← Exp.fromJson? obj
+    let vmap ← getFreeVars
 
-  | .ok ("FuncCheckSST", _) => do
+    let assertId ← coeWithState <| j.getNatUnderKey? "AssertId"
+    return Decl.assertion <| Assertion.mk s!"assert_{assertId}" vmap exp
+
+  | ("FuncCheckSST", _) => do
 
     let funcNameJson : Json ← j.getObjVal? "FnName"
     let funcName : String ← Json.getStr? funcNameJson
 
     throw s!"function {funcName} encountered: not yet implemented"
 
-  | .ok _ => throw "[Decl.fromJson?]: Expected one of { Assert, FuncCheckSST }, got something else"
-  | .error e => throw s!"[Decl.fromJson?]: {e}"
+  |  _ => throw "[Decl.fromJson?]: Expected one of { Assert, FuncCheckSST }, got something else"
 
-partial def Decls.fromFile? (path : String) : IO (Except String Decls) := do
+partial def Decls.fromFile? (path : String) : IO (Except String (List Decl)) := do
   let jsonStr ← IO.FS.readFile path
   let json ← IO.ofExcept <| Json.parse jsonStr
-  match Decls.fromJson? json (.Bool, Std.HashMap.empty) with
-  | .ok decls _ => return .ok decls
+  match Decl.fromJson? json default with
+  | .ok d st =>
+    let fns := st.fns.values.map (Decl.specFn ·)
+    return .ok (d :: fns)
   | .error e _ => return .error e
 
 /-
